

Deductive Program Verification using Hoare Logic

Andrei Arusoaie

What is Deductive Program Verification?

- ▶ Deductive program verification is a method to prove the correctness of programs using formal logic
- ▶ We need to specify what a program is supposed to do using logical formulas
- ▶ Examples: safety (no crashes), no arithmetic over/underflows, behavioral properties
- ▶ The program is verified by *proving* that these specifications (logical formulas) hold throughout the execution of the program

Why Deductive Program Verification is Useful?

- ▶ **Correctness:** Helps ensure that a program behaves as intended
- ▶ **Bug detection:** Formal methods can detect edge cases and bugs missed by testing
- ▶ Especially important for safety-critical systems (e.g., aviation, medical devices)
- ▶ **Drawback:** Requires higher expertise

(Floyd-)Hoare Logic

- ▶ Robert Floyd, 1967:
`https://people.eecs.berkeley.edu/~necula/Papers/
FloydMeaning.pdf`

(Floyd-)Hoare Logic

- ▶ Robert Floyd, 1967:
<https://people.eecs.berkeley.edu/~necula/Papers/FloydMeaning.pdf>
- ▶ Set the foundation of axiomatic semantics of classical programs

(Floyd-)Hoare Logic

- ▶ Robert Floyd, 1967:
<https://people.eecs.berkeley.edu/~necula/Papers/FloydMeaning.pdf>
- ▶ Set the foundation of axiomatic semantics of classical programs
- ▶ C. A. R. Hoare, 1969:
<https://dl.acm.org/doi/pdf/10.1145/363235.363259>
- ▶ Hoare is the inventor of quick sort, father of formal verification, Turing award winner 1980

Imperative Programming Language (IMP)

Arithmetic Expressions:

$\text{AExp} ::= \text{Var} \mid \text{Int} \mid \text{AExp} + \text{AExp} \mid \text{AExp} / \text{AExp}$

Boolean Expressions:

$\text{BExp} ::= \text{true} \mid \text{false} \mid \text{AExp} < \text{AExp}$
 $\mid \text{not BExp} \mid \text{BExp and BExp}$

Statements:

$\text{Stmt} ::= \text{Var} := \text{AExp}$
 $\mid \text{if BExp then Stmt else Stmt}$
 $\mid \text{while BExp do Stmt end}$
 $\mid \text{Stmt ; Stmt} \mid \text{skip}$

Deductive Program Verification Workflow

- ▶ **Step 1:** Write specifications for the program
- ▶ **Step 2:** Use Hoare logic to write the specs (e.g., *preconditions* and *postconditions*)
- ▶ **Step 3:** Generate verification conditions that prove the program's correctness
- ▶ **Step 4:** Use theorem provers to check if verification conditions hold

The sumPgm Program

Program:

```
sum := 0;  
i := 1;  
while (i < n + 1) do  
    sum := sum + i;  
    i := i + 1  
end
```

Input constraint: $n \geq 0$

The sumPgm Program

Program:

```
sum := 0;  
i := 1;  
while (i < n + 1) do  
    sum := sum + i;  
    i := i + 1  
end
```

Input constraint: $n \geq 0 \leftarrow$ called *precondition*

The sumPgm Program

Program:

```
sum := 0;  
i := 1;  
while (i < n + 1) do  
    sum := sum + i;  
    i := i + 1  
end
```

Input constraint: $n \geq 0 \leftarrow$ called *precondition*

Desired output property: $sum = \frac{n(n+1)}{2}$

The sumPgm Program

Program:

```
sum := 0;  
i := 1;  
while (i < n + 1) do  
    sum := sum + i;  
    i := i + 1  
end
```

Input constraint: $n \geq 0$ \leftarrow called *precondition*

Desired output property: $sum = \frac{n(n+1)}{2}$ \leftarrow called *postcondition*

Hoare Triples

- ▶ We can write specifications using Hoare triples:

$$\{P\} S \{Q\}$$

Hoare Triples

- ▶ We can write specifications using Hoare triples:

$$\{P\} S \{Q\}$$

- ▶ P is the precondition
- ▶ S is the program
- ▶ Q is the postcondition

Hoare Triples

- ▶ We can write specifications using Hoare triples:

$$\{P\} S \{Q\}$$

- ▶ P is the precondition
- ▶ S is the program
- ▶ Q is the postcondition

Hoare Triple for our program:

$$\{n \geq 0\} \text{sumPgm} \{sum = \frac{n(n+1)}{2}\}$$

Hoare Triples: Semantics

- ▶ How to establish the validity of a Hoare triple $\{P\} S \{Q\}$?

Hoare Triples: Semantics

- ▶ How to establish the validity of a Hoare triple $\{P\} S \{Q\}$?
- ▶ **Partial correctness:** If S is executed in a state satisfying P and the execution of S terminates, then the resulting program state satisfies Q
Valid (in the sense of partial correctness) triples are denoted:

$$\models \{P\} S \{Q\}$$

Hoare Triples: Semantics

- ▶ How to establish the validity of a Hoare triple $\{P\} S \{Q\}$?
- ▶ **Partial correctness:** If S is executed in a state satisfying P and the execution of S terminates, then the resulting program state satisfies Q
Valid (in the sense of partial correctness) triples are denoted:

$$\models \{P\} S \{Q\}$$

- ▶ **Total correctness:** If S is executed in a state satisfying P , then the execution of S terminates and the resulting program state satisfies Q (usually denoted by $[P] S [Q]$)
Valid (in the sense of total correctness) triples are denoted:

$$\models [P] S [Q]$$

Hoare Triples: Semantics

- ▶ How to establish the validity of a Hoare triple $\{P\} S \{Q\}$?
- ▶ **Partial correctness:** If S is executed in a state satisfying P and the execution of S terminates, then the resulting program state satisfies Q
Valid (in the sense of partial correctness) triples are denoted:

$$\models \{P\} S \{Q\}$$

- ▶ **Total correctness:** If S is executed in a state satisfying P , then the execution of S terminates and the resulting program state satisfies Q (usually denoted by $[P] S [Q]$)
Valid (in the sense of total correctness) triples are denoted:

$$\models [P] S [Q]$$

- ▶ We only discuss partial correctness (safety) in this material
Total correctness = Partial correctness + termination

A Few Interesting Examples

► $\{\text{true}\} \mathcal{S} \{Q\}$

A Few Interesting Examples

- ▶ $\{\text{true}\} \vdash \{Q\}$
- ▶ $\{P\} \vdash \{\text{true}\}$

A Few Interesting Examples

- ▶ $\{\text{true}\} S \{Q\}$
- ▶ $\{P\} S \{\text{true}\}$
- ▶ $[P] S [\text{true}]$

A Few Interesting Examples

- ▶ $\{\text{true}\} S \{Q\}$
- ▶ $\{P\} S \{\text{true}\}$
- ▶ $[P] S [\text{true}]$
- ▶ $\{\text{true}\} S \{\text{false}\}$

A Few Interesting Examples

- ▶ $\{\text{true}\} S \{Q\}$
- ▶ $\{P\} S \{\text{true}\}$
- ▶ $[P] S [\text{true}]$
- ▶ $\{\text{true}\} S \{\text{false}\}$
- ▶ $\{\text{false}\} S \{Q\}$

Which of the Following Triples are Valid?

► $\{i = 0\}$ while $i < n$ do $i := i + 1$ end $\{i = n\}$

Which of the Following Triples are Valid?

- ▶ $\{i = 0\}$ while $i < n$ do $i := i + 1$ end $\{i = n\}$
- ▶ $\{i = 0\}$ while $i < n$ do $i := i + 1$ end $\{i \geq n\}$

Which of the Following Triples are Valid?

► $\{i = 0\}$ while $i < n$ do $i := i + 1$ end $\{i = n\}$

► $\{i = 0\}$ while $i < n$ do $i := i + 1$ end $\{i \geq n\}$

► $\{i = 0 \wedge s = 0\}$

```
while i < n do
  i := i + 1;
  s := s + i
end
```

$\{2 \cdot s = n(n + 1)\}$

Proofs

- ▶ Challenge: how do we prove the validity of triples?

Proofs

- ▶ Challenge: how do we prove the validity of triples? We need a proof system!

Proofs

- ▶ Challenge: how do we prove the validity of triples? We need a proof system!
- ▶ We want a proof system to help with proving $\models \{P\} S \{Q\}$

Proofs

- ▶ Challenge: how do we prove the validity of triples? We need a proof system!
- ▶ We want a proof system to help with proving $\models \{P\} S \{Q\}$
- ▶ We use $\vdash \{P\} S \{Q\}$ to denote a *sequent*

Proofs

- ▶ Challenge: how do we prove the validity of triples? We need a proof system!
- ▶ We want a proof system to help with proving $\models \{P\} S \{Q\}$
- ▶ We use $\vdash \{P\} S \{Q\}$ to denote a *sequent*
- ▶ \vdash denotes syntactical calculus
- ▶ \models indicates semantic validity

Proof System Properties

- ▶ The proof system of Hoare Logic includes several proof rules which depend on the language constructs
- ▶ Hoare proved that his proof system is correct and (relatively-)complete
- ▶ Hoare also gave a sound and (relatively-)complete proof system that allows semi-mechanizing correctness proofs
- ▶ **Soundness:** If $\vdash \{P\} S \{Q\}$, then $\models \{P\} S \{Q\}$
- ▶ Unfortunately, completeness does **not** hold:
If $\models \{P\} S \{Q\}$, then $\vdash \{P\} S \{Q\}$

Inference Rules

- ▶ Proof rules in Hoare logic are written as inference rules:

$$\frac{\vdash \{P_1\} S_1 \{Q_1\} \quad \dots \quad \vdash \{P_n\} S_n \{Q_n\}}{\vdash \{P\} S \{Q\}}$$

- ▶ The sequents above the horizontal line are premises, while the sequent under the line is the conclusion
- ▶ The above rule says: if the sequents

$$\vdash \{P_1\} S_1 \{Q_1\}, \dots, \vdash \{P_n\} S_n \{Q_n\}$$

are provable in our proof system, then

$$\vdash \{P\} S \{Q\}$$

is also provable

- ▶ Rules with no hypotheses are called axioms

Understanding Proof Rule for Assignment

- ▶ There is one inference rule for every statement in the IMP language
- ▶ Assignments change the value of a variable in the state
- ▶ When $x := e$ is executed, what must be true before the assignment for a postcondition $\{Q\}$ to hold?
- ▶ Remark: $\{Q\}$ holds *after* the assignment!

Understanding Proof Rule for Assignment

- ▶ There is one inference rule for every statement in the IMP language
- ▶ Assignments change the value of a variable in the state
- ▶ When $x := e$ is executed, what must be true before the assignment for a postcondition $\{Q\}$ to hold?
- ▶ Remark: $\{Q\}$ holds *after* the assignment!
- ▶ So, e must be substituted for x in $\{Q\}$ before the assignment

Proof Rule for Assignment

$$\frac{\cdot}{\vdash \{Q[e/x]\} x := e \{Q\}}$$

- ▶ This means: if $\{Q[e/x]\}$ holds before the assignment, then after the assignment $x := e$, the postcondition $\{Q\}$ will hold
- ▶ Recall that $Q[e/x]$ is the notation for substitution: the postcondition Q with every occurrence of x replaced by the expression e

Example 1

Is this sequent valid: $\vdash \{\text{true}\} \ i := 2 \ \{i = 2\}$?

Example 1

Is this sequent valid: $\vdash \{\text{true}\} \ i := 2 \ \{i = 2\}$?

We use the assignment rule:

$$\frac{\cdot}{\vdash \{ Q[e/x] \} \ x := e \ \{ Q \}}$$

Example 1

Is this sequent valid: $\vdash \{\text{true}\} \ i := 2 \ \{i = 2\}$?

We use the assignment rule:

$$\frac{\cdot}{\vdash \{ Q[e/x] \} \ x := e \ \{ Q \}}$$

to obtain:

$$\vdash \{ i = 2[2/i] \} \ i := 2 \ \{ i = 2 \}$$

Example 1

Is this sequent valid: $\vdash \{\text{true}\} \ i := 2 \ \{i = 2\}$?

We use the assignment rule:

$$\frac{\cdot}{\vdash \{ Q[e/x] \} \ x := e \ \{ Q \}}$$

to obtain:

$$\frac{\cdot}{\vdash \{ i = 2[2/i] \} \ i := 2 \ \{ i = 2 \}}$$

We compute the substitution, and we get:

$$\frac{\cdot}{\vdash \{ 2 = 2 \} \ i := 2 \ \{ i = 2 \}}$$

Example 1

Is this sequent valid: $\vdash \{\text{true}\} \ i := 2 \ \{i = 2\}$?

We use the assignment rule:

$$\frac{\cdot}{\vdash \{ Q[e/x] \} \ x := e \ \{ Q \}}$$

to obtain:

$$\frac{\cdot}{\vdash \{ i = 2[2/i] \} \ i := 2 \ \{ i = 2 \}}$$

We compute the substitution, and we get:

$$\frac{\cdot}{\vdash \{ 2 = 2 \} \ i := 2 \ \{ i = 2 \}}$$

This results in:

$$\frac{\cdot}{\vdash \{ \text{true} \} \ i := 2 \ \{ i = 2 \}}$$

Example 2

Is this sequent valid: $\vdash \{i = k\} \ i := i + 1 \ \{i = k + 1\}$?

Example 2

Is this sequent valid: $\vdash \{i = k\} i := i + 1 \{i = k + 1\}$?

We use the assignment rule:

$$\frac{\cdot}{\vdash \{Q[e/x]\} x := e \{Q\}}$$

Example 2

Is this sequent valid: $\vdash \{i = k\} i := i + 1 \{i = k + 1\}$?

We use the assignment rule:

$$\frac{\cdot}{\vdash \{Q[e/x]\} x := e \{Q\}}$$

to obtain:

$$\vdash \{i = k + 1[i + 1/i]\} i := i + 1 \{i = k + 1\}$$

Example 2

Is this sequent valid: $\vdash \{i = k\} i := i + 1 \{i = k + 1\}$?

We use the assignment rule:

$$\frac{\cdot}{\vdash \{Q[e/x]\} x := e \{Q\}}$$

to obtain:

$$\frac{\cdot}{\vdash \{i = k + 1[i + 1/i]\} i := i + 1 \{i = k + 1\}}$$

We compute the substitution, and we get:

$$\frac{\cdot}{\vdash \{i + 1 = k + 1\} i := i + 1 \{i = k + 1\}}$$

Example 2

Is this sequent valid: $\vdash \{i = k\} i := i + 1 \{i = k + 1\}$?

We use the assignment rule:

$$\frac{\cdot}{\vdash \{Q[e/x]\} x := e \{Q\}}$$

to obtain:

$$\frac{\cdot}{\vdash \{i = k + 1[i + 1/i]\} i := i + 1 \{i = k + 1\}}$$

We compute the substitution, and we get:

$$\frac{\cdot}{\vdash \{i + 1 = k + 1\} i := i + 1 \{i = k + 1\}}$$

that is:

$$\frac{\cdot}{\vdash \{i = k\} i := i + 1 \{i = k + 1\}}$$

Example 3

Is this sequent valid: $\vdash \{s = k\} s := s + i \{s = k + i\}$?

Example 3

Is this sequent valid: $\vdash \{s = k\} s := s + i \{s = k + i\}$?

We use the assignment rule:

$$\frac{\cdot}{\vdash \{Q[e/x]\} x := e \{Q\}}$$

Example 3

Is this sequent valid: $\vdash \{s = k\} s := s + i \{s = k + i\}$?

We use the assignment rule:

$$\frac{\cdot}{\vdash \{Q[e/x]\} x := e \{Q\}}$$

to obtain:

$$\frac{\cdot}{\vdash \{s = k + i\} [s + i / s] s := s + i \{s = k + i\}}$$

Example 3

Is this sequent valid: $\vdash \{s = k\} s := s + i \{s = k + i\}$?

We use the assignment rule:

$$\frac{\cdot}{\vdash \{Q[e/x]\} x := e \{Q\}}$$

to obtain:

$$\frac{\cdot}{\vdash \{s = k + i\} [s + i / s] s := s + i \{s = k + i\}}$$

We compute the substitution, and we get:

$$\frac{\cdot}{\vdash \{s + i = k + i\} s := s + i \{s = k + i\}}$$

Example 3

Is this sequent valid: $\vdash \{s = k\} s := s + i \{s = k + i\}$?

We use the assignment rule:

$$\frac{\cdot}{\vdash \{Q[e/x]\} x := e \{Q\}}$$

to obtain:

$$\frac{\cdot}{\vdash \{s = k + i\} [s + i / s] s := s + i \{s = k + i\}}$$

We compute the substitution, and we get:

$$\frac{\cdot}{\vdash \{s + i = k + i\} s := s + i \{s = k + i\}}$$

Simplifying the equation, we obtain:

$$\frac{\cdot}{\vdash \{s = k\} s := s + i \{s = k + i\}}$$

Example 4

Is this sequent valid: $\vdash \{i \geq 0\} \ i := i + 1 \ \{i \geq 1\}$?

Example 4

Is this sequent valid: $\vdash \{i \geq 0\} \ i := i + 1 \ \{i \geq 1\}$?

We use the assignment rule:

$$\frac{\cdot}{\vdash \{ Q[e/x] \} \ x := e \ \{ Q \}}$$

Example 4

Is this sequent valid: $\vdash \{i \geq 0\} \ i := i + 1 \ \{i \geq 1\}$?

We use the assignment rule:

$$\frac{\cdot}{\vdash \{Q[e/x]\} \ x := e \ \{Q\}}$$

to obtain:

$$\vdash \{i \geq 1\} \ [i+1/i] \ i := i + 1 \ \{i \geq 1\}$$

Example 4

Is this sequent valid: $\vdash \{i \geq 0\} \ i := i + 1 \ \{i \geq 1\}$?

We use the assignment rule:

$$\frac{\cdot}{\vdash \{Q[e/x]\} \ x := e \ \{Q\}}$$

to obtain:

$$\frac{\cdot}{\vdash \{i \geq 1[i+1/i]\} \ i := i + 1 \ \{i \geq 1\}}$$

We compute the substitution, and we get:

$$\frac{\cdot}{\vdash \{i + 1 \geq 1\} \ i := i + 1 \ \{i \geq 1\}}$$

Example 4

Is this sequent valid: $\vdash \{i \geq 0\} \ i := i + 1 \ \{i \geq 1\}$?

We use the assignment rule:

$$\frac{\cdot}{\vdash \{Q[e/x]\} \ x := e \ \{Q\}}$$

to obtain:

$$\frac{\cdot}{\vdash \{i \geq 1 [i+1/i]\} \ i := i + 1 \ \{i \geq 1\}}$$

We compute the substitution, and we get:

$$\frac{\cdot}{\vdash \{i + 1 \geq 1\} \ i := i + 1 \ \{i \geq 1\}}$$

which simplifies to:

$$\frac{\cdot}{\vdash \{i \geq 0\} \ i := i + 1 \ \{i \geq 1\}}$$

Precondition Strengthening Rule

$$\frac{\vdash \{P'\} S \{Q\} \quad P \rightarrow P'}{\vdash \{P\} S \{Q\}}$$

Precondition Strengthening Rule

$$\frac{\vdash \{P'\} S \{Q\} \quad P \rightarrow P'}{\vdash \{P\} S \{Q\}}$$

- ▶ If $\vdash \{P'\} S \{Q\}$ and P implies P' , then $\vdash \{P\} S \{Q\}$ holds as well
- ▶ This rule is used to strengthen the precondition by making it *less strict* while maintaining the validity of the Hoare triple

Example: Precondition Strengthening

Is this sequent valid: $\vdash \{n > 0\} \ n := n + 1 \ \{n \geq 1\}$?

The precondition strengthening rule is:

$$\frac{\vdash \{P'\} \ S \ \{Q\} \quad P \rightarrow P'}{\vdash \{P\} \ S \ \{Q\}}$$

Here is the proof (which uses the assignment rule — see Example 4):

$$\frac{\vdash \{n \geq 0\} \ n := n + 1 \ \{n \geq 1\} \quad n > 0 \rightarrow n \geq 0}{\vdash \{n > 0\} \ n := n + 1 \ \{n \geq 1\}}$$

Proof Rule for Postcondition Weakening

- ▶ A dual rule for postconditions called *postcondition weakening*:

$$\frac{\vdash \{P\} S \{Q'\} \quad Q' \rightarrow Q}{\vdash \{P\} S \{Q\}}$$

- ▶ If we can prove postcondition Q' , we can always relax it to something weaker Q

Example: Postcondition Weakening

Is this sequent valid: $\vdash \{n > 0\} \ n := n + 1 \ \{n > 0\}$?

The postcondition weakening rule is:

$$\frac{\vdash \{P\} \ S \ \{Q'\} \quad Q' \rightarrow Q}{\vdash \{P\} \ S \ \{Q\}}$$

Here is the proof (which uses again the assignment rule):

$$\frac{\vdash \{n > 0\} \ n := n + 1 \ \{n \geq 1\} \quad n \geq 1 \rightarrow n > 0}{\vdash \{n > 0\} \ n := n + 1 \ \{n > 0\}}$$

Proof Rule for Composition

$$\frac{\vdash \{P\} S_1 \{Q\} \quad \vdash \{Q\} S_2 \{R\}}{\vdash \{P\} S_1 ; S_2 \{R\}}$$

- ▶ Remark: the postcondition of $\vdash \{P\} S_1 \{Q\}$ is the same as the precondition of $\vdash \{Q\} S_2 \{R\}$, which could be an issue in practice because they don't always match
- ▶ This could be a little restrictive, but precondition strengthening or postcondition weakening could be used to overcome this issue

Example: Composition Rule

Is this sequent valid: $\vdash \{\text{true}\} x := 2 ; y := x \{y = 2 \wedge x = 2\}$?

We use the composition rule:

$$\frac{\vdash \{P\} S_1 \{Q\} \quad \vdash \{Q\} S_2 \{R\}}{\vdash \{P\} S_1 ; S_2 \{R\}}$$

Here is the proof (which uses the assignment rule for both statements, individually):

$$\frac{\frac{\vdash \{\text{true}\} x := 2 \{x = 2\}}{\vdash \{\text{true}\} x := 2 ; y := x \{y = 2 \wedge x = 2\}} \quad \frac{\vdash \{x = 2\} y := x \{y = 2 \wedge x = 2\}}{\vdash \{\text{true}\} x := 2 ; y := x \{y = 2 \wedge x = 2\}}$$

Proof Rule for If Statements

$$\frac{\vdash \{P \wedge C\} S_1 \{Q\} \quad \vdash \{P \wedge \neg C\} S_2 \{Q\}}{\vdash \{P\} \text{ if } C \text{ then } S_1 \text{ else } S_2 \{Q\}}$$

- ▶ Suppose we know P holds before the if statement and want to show Q holds afterwards
- ▶ In the then branch, we want to show $\{P \wedge C\} S_1 \{Q\}$
- ▶ In the else branch, we want to show $\{P \wedge \neg C\} S_2 \{Q\}$

Example: Proof for If Statement

Is this sequent valid:

$$\vdash \{\text{true}\} \text{ if } x < 0 \text{ then } m := -x \text{ else } m := x \{m \geq 0\}?$$

We use the rule for if-statements:

$$\frac{\vdash \{P \wedge C\} S_1 \{Q\} \quad \vdash \{P \wedge \neg C\} S_2 \{Q\}}{\vdash \{P\} \text{ if } C \text{ then } S_1 \text{ else } S_2 \{Q\}}$$

Example: Proof for If Statement

Is this sequent valid:

$$\vdash \{\text{true}\} \text{ if } x < 0 \text{ then } m := -x \text{ else } m := x \{m \geq 0\}?$$

We use the rule for if-statements:

$$\frac{\vdash \{P \wedge C\} S_1 \{Q\} \quad \vdash \{P \wedge \neg C\} S_2 \{Q\}}{\vdash \{P\} \text{ if } C \text{ then } S_1 \text{ else } S_2 \{Q\}}$$

We show two branches:

$$\frac{\begin{array}{c} \dots \\ \vdash \{\text{true} \wedge x < 0\} m := -x \{m \geq 0\} \end{array} \quad \begin{array}{c} \dots \\ \vdash \{\text{true} \wedge \neg(x < 0)\} m := x \{m \geq 0\} \end{array}}{\vdash \{\text{true}\} \text{ if } x < 0 \text{ then } m := -x \text{ else } m := x \{m \geq 0\}}$$

Example: Proof for If Statement (Complete)

The proof of

$\vdash \{\text{true}\} \text{ if } x < 0 \text{ then } m := -x \text{ else } m := x \{m \geq 0\}$:

$$\frac{\frac{\vdash \{-x \geq 0\} \quad m := -x \quad \vdash \{m \geq 0\} \quad \text{true} \wedge (x < 0) \rightarrow -x \geq 0}{\vdash \{\text{true} \wedge x < 0\} \quad m := -x \quad \vdash \{m \geq 0\}} \quad \frac{\vdash \{x \geq 0\} \quad m := x \quad \vdash \{m \geq 0\} \quad \text{true} \wedge \neg (x < 0) \rightarrow x \geq 0}{\vdash \{\text{true} \wedge \neg (x < 0)\} \quad m := x \quad \vdash \{m \geq 0\}}}{\vdash \{\text{true}\} \text{ if } x < 0 \text{ then } m := -x \text{ else } m := x \{m \geq 0\}}$$

Proof Rule for While and Loop Invariants

Proof Rule for While:

$$\frac{\vdash \{I \wedge C\} S \{I\}}{\vdash \{I\} \text{ while } C \text{ do } S \text{ end } \{I \wedge \neg C\}}$$

- ▶ To understand the proof rule for while loops, we first need the concept of a **loop invariant**
- ▶ A loop invariant I ...
 1. ... holds before the loop starts and after the loop ends
 2. ... holds after every iteration of the loop

Example: Proof for While Statement

Is this sequent valid:

$$\vdash \{i = 0\} \text{ while } (i < n) \text{ do } i := i + 1 \text{ end } \{i = n\}?$$

Note: n is a natural number

$$\frac{\vdash \{I \wedge i < n\} i := i + 1 \{I\}}{\vdash \{I\} \text{ while } (i < n) \text{ do } i := i + 1 \text{ end } \{I \wedge \neg (i < n)\}}$$

In this case, the loop invariant is $I = (i \leq n)$:

Example: Proof for While Statement

Is this sequent valid:

$$\vdash \{i = 0\} \text{ while } (i < n) \text{ do } i := i + 1 \text{ end } \{i = n\}?$$

Note: n is a natural number

$$\frac{\vdash \{I \wedge i < n\} i := i + 1 \{I\}}{\vdash \{I\} \text{ while } (i < n) \text{ do } i := i + 1 \text{ end } \{I \wedge \neg(i < n)\}}$$

In this case, the loop invariant is $I = (i \leq n)$:

$$\begin{array}{c} \frac{}{\vdash \{i + 1 \leq n\} i := i + 1 \{i \leq n\}} \quad i \leq n \wedge i < n \rightarrow i + 1 \leq n \\ \hline \vdash \{i \leq n \wedge i < n\} i := i + 1 \{i \leq n\} \\ \hline \vdash \{i \leq n\} \text{ while } (i < n) \text{ do } i := i + 1 \text{ end } \{i \leq n \wedge \neg(i < n)\} \quad i \leq n \wedge \neg(i < n) \rightarrow i = n \\ \hline \vdash \{i \leq n\} \text{ while } (i < n) \text{ do } i := i + 1 \text{ end } \{i = n\} \quad i = 0 \rightarrow i \leq n \\ \hline \vdash \{i = 0\} \text{ while } (i < n) \text{ do } i := i + 1 \text{ end } \{i = n\} \end{array}$$

Proof of Invariant for While Loop — Part I

We prove that $i \leq n$ is the invariant for:

`while ($i < n$) do $i := i + 1$ end`

Remark: $I = (i \leq n)$ must be true before and after each iteration.

The sequent we proved:

$$\vdash \{i = 0\} \text{ while } (i < n) \text{ do } i := i + 1 \text{ end } \{i = n\}$$

The invariant holds before the loop: The precondition $i = 0$ implies $i \leq n$

The invariant is preserved by the loop body:

We need to prove the sequent:

$$\vdash \{i \leq n \wedge i < n\} i := i + 1 \{i \leq n\}$$

Proof of Invariant for While Loop — Part II

The proof is below:

$$\frac{\cdot \quad \vdash \{i + 1 \leq n\} \ i := i + 1 \ \{i \leq n\} \quad (i \leq n \wedge i < n) \rightarrow i + 1 \leq n}{\vdash \{i \leq n \wedge i < n\} \ i := i + 1 \ \{i \leq n\}}$$

Therefore, $i \leq n$ still holds after the iteration, including the last iteration.

At the end of the loop, the invariant $i \leq n$ holds, but the condition of the loop does not hold anymore; so, $\neg(i < n)$ holds, that is, $i \geq n$.

From $i \leq n$ and $i \geq n$ we have $i = n$.

Summary of Hoare Logic Proof Rules

Assignment

$$\frac{}{\vdash \{Q[e/x]\} x := e \{Q\}}$$

Precondition Strengthening

$$\frac{\vdash \{P'\} S \{Q\} \quad P \rightarrow P'}{\vdash \{P\} S \{Q\}}$$

Postcondition Weakening

$$\frac{\vdash \{P\} S \{Q'\} \quad Q' \rightarrow Q}{\vdash \{P\} S \{Q\}}$$

Composition

$$\frac{\vdash \{P\} S_1 \{Q\} \quad \vdash \{Q\} S_2 \{R\}}{\vdash \{P\} S_1; S_2 \{R\}}$$

If

$$\frac{\vdash \{P \wedge C\} S_1 \{Q\} \quad \vdash \{P \wedge \neg C\} S_2 \{Q\}}{\vdash \{P\} \text{if } C \text{ then } S_1 \text{ else } S_2 \{Q\}}$$

While

$$\frac{\vdash \{I \wedge C\} S \{I\}}{\vdash \{I\} \text{while } C \text{ do } S \text{ end } \{I \wedge \neg C\}}$$

Soundness

- ▶ It can be shown that the proof rules for Hoare logic are sound:

$$\text{If } \vdash \{P\} S \{Q\}, \text{ then } \models \{P\} S \{Q\}$$

- ▶ This means that if $\vdash \{P\} S \{Q\}$ is provable using the proof rules, then $\models \{P\} S \{Q\}$ — the triple is semantically valid
- ▶ Completeness of proof rules means that if $\{P\} S \{Q\}$ is a semantically valid Hoare triple, then it can be proven using our proof rules, i.e.,

$$\text{If } \models \{P\} S \{Q\}, \text{ then } \vdash \{P\} S \{Q\}$$

- ▶ Unfortunately, completeness does **not** hold!

Relative Completeness

- ▶ The rules for precondition strengthening and postcondition weakening contain implications $\varphi \rightarrow \varphi'$
- ▶ There are valid implications that cannot be proven (due to Peano Arithmetic which is incomplete)
- ▶ The rules still provide an important guarantee, called *relative completeness*:

If we have an oracle for deciding whether an implication $\varphi \Rightarrow \varphi'$ holds, then any valid Hoare triple can be proven using our proof rules.

The sum Program in Dafny

```
1  method mysum(n: nat) returns (sum: int)
2      requires n >= 0
3      ensures sum == n * (n + 1) / 2
4  {
5      sum := 0;
6      var i := 1;
7
8      while i < n + 1
9          invariant 1 <= i <= n + 1
10         invariant sum == i * (i - 1) / 2
11     {
12         sum := sum + i;
13         i := i + 1;
14     }
15 }
```

This is a direct translation of our Hoare Logic proof into executable, verified code!

What Dafny Automatically Verifies

When you compile this Dafny program, it automatically:

1. **Initial State:** Checks that the invariant holds after initialization
 - ▶ After `sum := 0; i := 1`, does the invariant hold?
2. **Preservation:** Verifies that the loop body preserves the invariant
 - ▶ If `invariant \wedge condition` holds before, does invariant hold after?
3. **Postcondition:** Confirms that `invariant \wedge \neg condition` implies postcondition
 - ▶ invariant implies `sum == n*(n+1)/2`

Summary

- ▶ Deductive Program Verification — a method to prove program correctness using formal logic
- ▶ Hoare Logic — a system to reason about program correctness using Hoare triples $\{P\} S \{Q\}$
- ▶ Partial Correctness vs Total Correctness (termination!)
- ▶ The Hoare Logic Proof System: A set of rules for proving the validity of Hoare triples
- ▶ Soundness and Relative Completeness